Peterson.thy
@@ -3,64 +3,72 @@ theory Peterson
 begin
 
 datatype globals = flag0 | flag1 | turn
-record aux = 
-  a0 :: bool 
-  a1 :: bool
+record aux = S :: bool
+
+text \<open>
+S indicates the conditions under which Thread 0 would have to wait.
+Mutual exclusion is demonstrated by ensuring Thread 0 requires a false S,
+whilst Thread 1 requires a true S.
+\<close>
 
 lemma peterson0:
   "FNBEGIN
-    R: \<^sup>1\<lbrakk>flag0\<rbrakk> = \<^sup>2\<lbrakk>flag0\<rbrakk> \<and> (\<^sup>1\<lbrakk>turn\<rbrakk> \<longrightarrow> \<^sup>2\<lbrakk>turn\<rbrakk>)
-    G: \<^sup>1\<lbrakk>flag1\<rbrakk> = \<^sup>2\<lbrakk>flag1\<rbrakk> \<and> (\<^sup>1\<lbrakk>turn\<rbrakk> \<longrightarrow> \<^sup>2\<lbrakk>turn\<rbrakk>)
+    R: (\<^sup>1\<lbrakk>flag0\<rbrakk> \<longrightarrow> \<^sup>2\<^sup>aS \<longrightarrow> \<^sup>1\<^sup>aS) \<and> \<^sup>1\<lbrakk>flag0\<rbrakk> = \<^sup>2\<lbrakk>flag0\<rbrakk> \<and> (\<^sup>2\<lbrakk>turn\<rbrakk> = \<^sup>1\<lbrakk>turn\<rbrakk> \<or> (\<^sup>1\<lbrakk>turn\<rbrakk> \<and> \<not>\<^sup>2\<lbrakk>turn\<rbrakk> \<and> (\<^sup>1\<lbrakk>flag0\<rbrakk> \<longrightarrow> \<not>\<^sup>2\<^sup>aS)))
+    G: (\<^sup>1\<lbrakk>flag1\<rbrakk> \<longrightarrow> \<^sup>1\<^sup>aS \<longrightarrow> \<^sup>2\<^sup>aS) \<and> \<^sup>1\<lbrakk>flag1\<rbrakk> = \<^sup>2\<lbrakk>flag1\<rbrakk> \<and> (\<^sup>2\<lbrakk>turn\<rbrakk> = \<^sup>1\<lbrakk>turn\<rbrakk> \<or> (\<not>\<^sup>1\<lbrakk>turn\<rbrakk> \<and> \<^sup>2\<lbrakk>turn\<rbrakk> \<and> (\<^sup>1\<lbrakk>flag1\<rbrakk> \<longrightarrow> \<^sup>2\<^sup>aS)))
     P: True
     {
       \<lbrakk>flag0\<rbrakk> := #True;
-      fence;
-      \<lbrakk>turn\<rbrakk> := #True;
-      fence;
+      \<lbrakk>turn\<rbrakk> := #True :\<^sub>a \<^sup>aS := True;
       do
-        \<^bold>r0 := \<lbrakk>flag1\<rbrakk>, \<^sup>aa0 := \<^sup>0\<lbrakk>flag1\<rbrakk>;
+        \<^bold>r0 := \<lbrakk>flag1\<rbrakk> :\<^sub>a \<^sup>aS := (\<^sup>aS \<and> \<^sup>0\<lbrakk>flag1\<rbrakk>);
         \<^bold>r1 := \<lbrakk>turn\<rbrakk>
+      inv \<lbrace>\<^sup>0\<lbrakk>flag0\<rbrakk> \<and> (\<^sup>aS \<longrightarrow> \<^sup>0\<lbrakk>turn\<rbrakk>)\<rbrace>
       while (\<^bold>r0 && \<^bold>r1);
-      Skip;
+      \<lbrace>\<not>\<^sup>aS\<rbrace> skip;
       \<lbrakk>flag0\<rbrakk> := #False
     }
     Q: True
   FNEND" 
-  apply(unfold fn_valid.simps, intro conjI)
-
+  apply (unfold fn_valid.simps, intro conjI)
+  
+  (* Stability of Q + Wellformedness of R & G *)
   apply (auto simp: step\<^sub>t_def stable_def reflexive_def transitive_def)[4]
 
-  apply (clarsimp simp: aux_upd_def step_def glb_def wp\<^sub>r_def)
+  (* Guarantees of each atomic action *)
+  apply (clarsimp simp: aux_upd_def step_def glb_def wp\<^sub>r_def st_upd_def)
 
-  sorry
-
+  (* WP reasoning *)
+  by (simp add: c_and_def test_def, intro conjI impI; 
+      clarsimp simp: stabilize_def st_upd_def glb_def rg_def aux_upd_def; metis)
 
 lemma peterson1:
   "FNBEGIN
-    R: True
-    G: \<^sup>1\<lbrakk>flag0\<rbrakk> = \<^sup>2\<lbrakk>flag0\<rbrakk> \<and> (\<^sup>1\<lbrakk>turn\<rbrakk> = 0 \<longrightarrow> \<^sup>2\<lbrakk>turn\<rbrakk> = 0)
+    R: (\<^sup>1\<lbrakk>flag1\<rbrakk> \<longrightarrow> \<^sup>1\<^sup>aS \<longrightarrow> \<^sup>2\<^sup>aS) \<and> \<^sup>1\<lbrakk>flag1\<rbrakk> = \<^sup>2\<lbrakk>flag1\<rbrakk> \<and> (\<^sup>2\<lbrakk>turn\<rbrakk> = \<^sup>1\<lbrakk>turn\<rbrakk> \<or> (\<not>\<^sup>1\<lbrakk>turn\<rbrakk> \<and> \<^sup>2\<lbrakk>turn\<rbrakk> \<and> (\<^sup>1\<lbrakk>flag1\<rbrakk> \<longrightarrow> \<^sup>2\<^sup>aS)))
+    G: (\<^sup>1\<lbrakk>flag0\<rbrakk> \<longrightarrow> \<^sup>2\<^sup>aS \<longrightarrow> \<^sup>1\<^sup>aS) \<and> \<^sup>1\<lbrakk>flag0\<rbrakk> = \<^sup>2\<lbrakk>flag0\<rbrakk> \<and> (\<^sup>2\<lbrakk>turn\<rbrakk> = \<^sup>1\<lbrakk>turn\<rbrakk> \<or> (\<^sup>1\<lbrakk>turn\<rbrakk> \<and> \<not>\<^sup>2\<lbrakk>turn\<rbrakk> \<and> (\<^sup>1\<lbrakk>flag0\<rbrakk> \<longrightarrow> \<not>\<^sup>2\<^sup>aS)))
     P: True
     {
-      \<lbrakk>flag1\<rbrakk> := true;
-      \<lbrakk>turn\<rbrakk> := #0;
-      while (\<lbrakk>flag0\<rbrakk> == true) && (\<lbrakk>turn\<rbrakk> == #0)
+      \<lbrakk>flag1\<rbrakk> := #True;
+      \<lbrakk>turn\<rbrakk> := #False :\<^sub>a \<^sup>aS := False;
       do
-        Skip
-      od;
-      \<^bold>r0 := \<^bold>r2;
-      \<lbrakk>flag1\<rbrakk> := false
+        \<^bold>r0 := \<lbrakk>flag0\<rbrakk> :\<^sub>a \<^sup>aS := (\<^sup>aS \<or> \<not>\<^sup>0\<lbrakk>flag0\<rbrakk>);
+        \<^bold>r1 := (!\<lbrakk>turn\<rbrakk>)
+      inv \<lbrace>\<^sup>0\<lbrakk>flag1\<rbrakk> \<and> (\<^sup>0\<lbrakk>turn\<rbrakk> \<longrightarrow> \<^sup>aS)\<rbrace>
+      while (\<^bold>r0 && \<^bold>r1);
+      \<lbrace>\<^sup>aS\<rbrace> skip;
+      \<lbrakk>flag1\<rbrakk> := #False
     }
     Q: True
   FNEND" 
   apply(unfold fn_valid.simps, intro conjI)
 
+  (* Stability of Q + Wellformedness of R & G *)
   apply (auto simp: step\<^sub>t_def stable_def reflexive_def transitive_def)[4]
 
-  apply (clarsimp simp: step_def glb_def wp\<^sub>r_def)
+  (* Guarantees of each atomic action *)
+  apply (clarsimp simp: aux_upd_def step_def glb_def wp\<^sub>r_def st_upd_def)
 
-  apply (simp add: stabilize_def assert_def)
-
-  done
-
+  (* WP reasoning *)
+  by (simp add: c_and_def c_neg_def test_def, intro conjI impI; 
+      clarsimp simp: stabilize_def st_upd_def glb_def rg_def aux_upd_def; metis)
 
 end
