PetersonLitmus.thy
@@ -1,0 +1,67 @@
+theory PetersonLitmus
+  imports SimAsm_Syntax
+begin
+
+datatype globals = X | Y | T
+record aux = S :: bool
+
+lemma thread0:
+  "FNBEGIN
+    R: (\<^sup>1\<lbrakk>X\<rbrakk> \<longrightarrow> \<^sup>2\<^sup>aS \<longrightarrow> \<^sup>1\<^sup>aS) \<and> \<^sup>1\<lbrakk>X\<rbrakk> = \<^sup>2\<lbrakk>X\<rbrakk> \<and> (\<^sup>2\<lbrakk>T\<rbrakk> = \<^sup>1\<lbrakk>T\<rbrakk> \<or> (\<^sup>1\<lbrakk>T\<rbrakk> \<and> \<not> \<^sup>2\<lbrakk>T\<rbrakk> \<and> (\<^sup>1\<lbrakk>X\<rbrakk> \<longrightarrow> \<not>\<^sup>2\<^sup>aS)))
+    G: (\<^sup>1\<lbrakk>Y\<rbrakk> \<longrightarrow> \<^sup>1\<^sup>aS \<longrightarrow> \<^sup>2\<^sup>aS) \<and> \<^sup>1\<lbrakk>Y\<rbrakk> = \<^sup>2\<lbrakk>Y\<rbrakk> \<and> (\<^sup>2\<lbrakk>T\<rbrakk> = \<^sup>1\<lbrakk>T\<rbrakk> \<or> (\<not>\<^sup>1\<lbrakk>T\<rbrakk> \<and> \<^sup>2\<lbrakk>T\<rbrakk> \<and> (\<^sup>1\<lbrakk>Y\<rbrakk> \<longrightarrow> \<^sup>2\<^sup>aS)))
+    P: True
+    {
+      \<lbrakk>X\<rbrakk> := #True;
+      \<lbrakk>T\<rbrakk> := #True :\<^sub>a \<^sup>aS := True;
+      \<^bold>r0 := \<lbrakk>Y\<rbrakk> :\<^sub>a \<^sup>aS := (\<^sup>aS \<and> \<^sup>0\<lbrakk>Y\<rbrakk>);
+      \<^bold>r1 := \<lbrakk>T\<rbrakk>
+    }
+    Q: (\<^sup>0\<lbrakk>X\<rbrakk> \<and> (\<^sup>aS \<longrightarrow> \<^sup>0\<^bold>r(0 :: nat) \<and> \<^sup>0\<^bold>r1))
+  FNEND" 
+  apply (unfold fn_valid.simps, intro conjI)
+
+  (* Stability of Q *)
+  apply (auto simp: glb_def step\<^sub>t_def stable_def)[1]
+
+  (* Wellformedness of R & G *)
+  apply (auto simp: transitive_def reflexive_def)[3]
+
+  (* Guarantees of each atomic action *)
+  apply (auto simp: wp\<^sub>r_def st_upd_def step_def glb_def aux_upd_def)[1]
+
+  apply simp
+  apply (clarsimp simp: stabilize_def st_upd_def glb_def aux_upd_def rg_def)
+  by (meson less_numeral_extra(3))
+
+lemma thread1:
+  "FNBEGIN
+    R: (\<^sup>1\<lbrakk>Y\<rbrakk> \<longrightarrow> \<^sup>1\<^sup>aS \<longrightarrow> \<^sup>2\<^sup>aS) \<and> \<^sup>1\<lbrakk>Y\<rbrakk> = \<^sup>2\<lbrakk>Y\<rbrakk> \<and> (\<^sup>2\<lbrakk>T\<rbrakk> = \<^sup>1\<lbrakk>T\<rbrakk> \<or> (\<not>\<^sup>1\<lbrakk>T\<rbrakk> \<and> \<^sup>2\<lbrakk>T\<rbrakk> \<and> (\<^sup>1\<lbrakk>Y\<rbrakk> \<longrightarrow> \<^sup>2\<^sup>aS)))
+    G: (\<^sup>1\<lbrakk>X\<rbrakk> \<longrightarrow> \<^sup>2\<^sup>aS \<longrightarrow> \<^sup>1\<^sup>aS) \<and> \<^sup>1\<lbrakk>X\<rbrakk> = \<^sup>2\<lbrakk>X\<rbrakk> \<and> (\<^sup>2\<lbrakk>T\<rbrakk> = \<^sup>1\<lbrakk>T\<rbrakk> \<or> (\<^sup>1\<lbrakk>T\<rbrakk> \<and> \<not> \<^sup>2\<lbrakk>T\<rbrakk> \<and> (\<^sup>1\<lbrakk>X\<rbrakk> \<longrightarrow> \<not>\<^sup>2\<^sup>aS)))
+    P: True
+    {
+      \<lbrakk>Y\<rbrakk> := #True;
+      \<lbrakk>T\<rbrakk> := #False :\<^sub>a \<^sup>aS := False;
+      \<^bold>r0 := \<lbrakk>X\<rbrakk> :\<^sub>a \<^sup>aS := (\<^sup>aS \<or> \<not>\<^sup>0\<lbrakk>X\<rbrakk>);
+      \<^bold>r1 := (!\<lbrakk>T\<rbrakk>)
+    }
+    Q: (\<^sup>0\<lbrakk>Y\<rbrakk> \<and> (\<not>\<^sup>aS \<longrightarrow> \<^sup>0\<^bold>r(0 :: nat) \<and> \<^sup>0\<^bold>r1))
+  FNEND" 
+  apply (unfold fn_valid.simps, intro conjI)
+
+  (* Stability of Q *)
+  apply (auto simp: glb_def step\<^sub>t_def stable_def)[1]
+
+  (* Wellformedness of R & G *)
+  apply (auto simp: transitive_def reflexive_def)[3]
+
+  (* Guarantees of each atomic action *)
+  apply (auto simp: wp\<^sub>r_def st_upd_def step_def glb_def aux_upd_def)[1]
+
+  apply simp
+  apply (clarsimp simp: stabilize_def st_upd_def glb_def aux_upd_def rg_def c_neg_def)
+  apply (intro conjI impI)
+  defer 1
+  apply (meson less_numeral_extra(3))
+  by auto
+
+end
